proof/refine/RISCV64/Arch_R.thy
@@ -9,7 +9,7 @@
 *)
 
 theory Arch_R
-imports Untyped_R ArchFinalise_R
+imports ArchUntyped_R ArchFinalise_R
 begin
 
 unbundle l4v_word_context
